ok

Lamcalc/Basics.lean
@@ -1,58 +1,162 @@
-class Ids (t : Type) where
-  ids : Nat -> t
+import Lamcalc.Attr
 
-class Rename (t : Type) where
-  rename : (Nat -> Nat) -> t -> t
+-------------------------------------------------------------------------------------------------
 
-class Subst (t : Type) where
-  subst : (Nat -> t) -> t -> t
+section Definitions
+
+abbrev Var := Nat
+
+class Ids (T : Type) where
+  ids : Var -> T
+
+class Rename (T : Type) where
+  rename : (Var -> Var) -> T -> T
+
+class Subst (T : Type) where
+  subst : (Var -> T) -> T -> T
 
 export Ids (ids)
 export Rename (rename)
 export Subst (subst)
 
-@[simp]
-def scons {T} (s : T) (σ : Nat -> T) : Nat -> T
+@[asimp]def scons {T} (s : T) (σ : Var -> T) : Var -> T
   | 0 => s
   | x+1 => σ x
 
-@[simp]
-def funcomp {A B C} (f : A -> B) (g : B -> C) : A -> C :=
+@[asimp]def funcomp {A B C} (f : A -> B) (g : B -> C) : A -> C :=
   fun x => g (f x)
 
-def scomp {T} [Subst T] (f g : Nat -> T) : Nat -> T :=
+def scomp {T} [Subst T] (f g : Var -> T) : Var -> T :=
   funcomp f (subst g)
 
-infixl:56 " @@@ " => funcomp
-infixl:56 " @@ " => scomp
+infixl:56 " >>> " => funcomp
+infixl:56 " >> " => scomp
 infixr:55 " .: " => scons
 notation:max s:2 ".[" σ:2 "]" => subst σ s
 notation:max s:2 ".[" t:2 "/]" => subst (t .: ids) s
 
-def ren {T} [Ids T] (ξ : Nat -> Nat) : Nat -> T :=
-  ξ @@@ ids
+def ren {T} [Ids T] (ξ : Var -> Var) : Var -> T :=
+  ξ >>> ids
 
-def shift {T} [Ids T] : Nat -> T :=
+def shift {T} [Ids T] : Var -> T :=
   ren Nat.succ
 
-def upren (ξ : Nat -> Nat) : Nat -> Nat :=
-  0 .: ξ @@@ Nat.succ
+def upren (ξ : Var -> Var) : Var -> Var :=
+  0 .: ξ >>> Nat.succ
 
-def up {T} [Ids T] [Rename T] (σ : Nat -> T) : Nat -> T :=
-  ids 0 .: (σ @@@ rename Nat.succ)
+def up {T} [Ids T] [Rename T] (σ : Var -> T) : Var -> T :=
+  ids 0 .: (σ >>> rename Nat.succ)
 
-def upn {T} [Ids T] [Rename T] (n : Nat) : (Nat -> T) -> Nat -> T :=
+def upn {T} [Ids T] [Rename T] (n : Var) : (Var -> T) -> Var -> T :=
   n.repeat up
 
-@[simp] theorem upren0 (ξ : Nat -> Nat) : upren ξ 0 = 0 := by rfl
-@[simp] theorem up0 {T} [Ids T] [Rename T] (σ : Nat -> T) : up σ 0 = ids 0 := by rfl
-@[simp] theorem up1 {T} [Ids T] [Rename T] (σ : Nat -> T) : up σ (n + 1) = rename Nat.succ (σ n) := by rfl
-@[simp] theorem upn0 {T} [Ids T] [Rename T] σ : @upn T _ _ 0 σ = σ := by rfl
-@[simp] theorem upn1 {T} [Ids T] [Rename T] (n : Nat) σ : @upn T _ _ (n + 1) σ = upn n (up σ) := by
-  induction n with
-  | zero => simp[upn, Nat.repeat]
-  | succ n ih =>
-    simp[upn, Nat.repeat]
-    rw [<-upn]
-    rw [<-ih]
-    simp[upn, Nat.repeat]
+@[asimp]theorem scomp0 {T} [Subst T] (f g : Var -> T) (x : Var) :
+  (f >> g) x = (f x).[g] := by rfl
+@[asimp]theorem scons0 {T} (s : T) (σ : Var -> T) : (s .: σ) 0 = s := by rfl
+@[asimp]theorem scons1 {T} (s : T) (σ : Var -> T) (x : Var) : (s .: σ) x.succ = σ x := by rfl
+@[asimp]theorem ren0 {T} [Ids T] (x : Var) (ξ : Var -> Var) : ren ξ x = @ids T _ (ξ x) := by rfl
+@[asimp]theorem upren0 (ξ : Var -> Var) : upren ξ 0 = 0 := by rfl
+@[asimp]theorem upren1 (ξ : Var -> Var) : upren ξ (n + 1) = (ξ >>> Nat.succ) n := by
+  simp[upren, scons]
+@[asimp]theorem up0 {T} [Ids T] [Rename T] (σ : Var -> T) : up σ 0 = ids 0 := by rfl
+@[asimp]theorem up1 {T} [Ids T] [Rename T] (σ : Var -> T) : up σ (n + 1) = rename Nat.succ (σ n) := by rfl
+@[asimp]theorem upn0 {T} [Ids T] [Rename T] (σ : Var -> T) : upn 0 σ = σ := by rfl
+@[asimp]theorem upn1 {T} [Ids T] [Rename T] (n : Var) σ : @upn T _ _ (n + 1) σ = up (upn n σ) := by
+  simp[upn, Nat.repeat]
+
+@[asimp]theorem id_comp (f : A -> B) : id >>> f = f := by rfl
+@[asimp]theorem comp_id (f : A -> B) : f >>> id = f := by rfl
+@[asimp]theorem comp_assoc (f : A -> B) (g : B -> C) (h : C -> D) :
+  (f >>> g) >>> h = f >>> (g >>> h) := by rfl
+
+@[asimp]theorem lift0 : (.+0) = id := by rfl
+@[asimp]theorem lift_scons x (f : Var -> T) (n : Var) :
+  (.+n.succ) >>> (x .: f) = (.+n) >>> f := by
+  funext x0; simp[scons, asimp]
+
+section Definitions
+
+-------------------------------------------------------------------------------------------------
+
+section Lemmas
+
+class SubstLemmas (T : Type) [Ids T] [Rename T] [Subst T] where
+  rename_subst (ξ : Var -> Var) (m : T) : rename ξ m = m.[ren ξ]
+  subst_id (m : T) : m.[ids] = m
+  id_subst (σ : Var -> T) (x : Var) : (ids x).[σ] = σ x
+  subst_comp (σ τ : Var -> T) (s : T) : s.[σ].[τ] = s.[σ >> τ]
+
+set_option linter.unusedSectionVars false
+variable {T : Type} [Ids T] [Rename T] [Subst T] [lemmas: SubstLemmas T]
+
+@[asimp]theorem rename_subst :
+  ∀ (ξ : Var -> Var) (m : T), rename ξ m = m.[ren ξ] := lemmas.rename_subst
+
+@[asimp]theorem subst_id :
+  ∀ (m : T), m.[ids] = m := lemmas.subst_id
+
+@[asimp]theorem id_subst :
+  ∀ (σ : Var -> T) (x : Var), (ids x).[σ] = σ x := lemmas.id_subst
+
+@[asimp]theorem subst_comp :
+  ∀ (σ τ : Var -> T) (s : T), s.[σ].[τ] = s.[σ >> τ] := lemmas.subst_comp
+
+@[asimp]theorem up_shift (σ : Var -> T) :
+  up σ = ids 0 .: (σ >> shift) := by
+  simp[up, asimp]
+  funext x
+  cases x with
+  | zero => simp[asimp]
+  | succ => simp[shift, scomp, asimp]
+
+@[asimp]theorem ids_comp (σ : Var -> T) : ids >> σ = σ := by
+  funext x
+  simp[scomp, asimp]
+
+@[asimp]theorem ids_shift : (@ids T _ 0) .: shift = ids := by
+  funext x
+  cases x with
+  | zero => simp[asimp]
+  | succ => simp[scons, shift, ren, funcomp]
+
+@[asimp]theorem shift_scomp (m : T) (σ : Var -> T) :
+  shift >> (m .: σ) = σ := by
+  funext x
+  simp[scomp, shift, ren, asimp]
+
+@[asimp]theorem ids0_scons (σ : Var -> T) :
+  (ids 0).[σ] .: (shift >> σ) = σ := by
+  funext x
+  simp[scons]
+  cases x with
+  | zero => simp[asimp]
+  | succ => simp[scomp, shift, ren, asimp]
+
+@[asimp]theorem comp_ids (σ : Var -> T) : σ >> ids = σ := by
+  funext x
+  simp[scomp, funcomp, asimp]
+
+@[asimp]theorem scons_scomp m (σ τ : Var -> T) :
+  (m .: σ) >> τ = m.[τ] .: σ >> τ := by
+  funext x
+  cases x with
+  | zero => simp[scomp, funcomp, scons]
+  | succ => simp[scomp, funcomp, scons]
+
+@[asimp]theorem scomp_assoc (σ τ θ : Var -> T) :
+  (σ >> τ) >> θ = σ >> (τ >> θ) := by
+  funext x
+  simp[scomp, funcomp, asimp]
+
+end Lemmas
+
+syntax "asimp" ("[" ident,+ "]")? ("at" ident)? : tactic
+macro_rules
+| `(tactic| asimp) =>
+  `(tactic| simp[asimp]; repeat rw [<-up_shift])
+| `(tactic| asimp[$[$x:ident],*]) =>
+  `(tactic| simp[$[$x:ident],*, asimp]; repeat rw [<-up_shift])
+| `(tactic| asimp at $h:ident) =>
+  `(tactic| simp[asimp] at $h:ident; repeat rw [<-up_shift] at $h:ident)
+| `(tactic| asimp[$[$x:ident],*] at $h:ident) =>
+  `(tactic| simp[$[$x:ident],*, asimp] at $h:ident; repeat rw [<-up_shift] at $h:ident)
