Lamcalc/Syntax.lean
@@ -5,7 +5,7 @@ inductive ty where
 | unit
 
 inductive tm where
-| var : Nat -> tm
+| var : Var -> tm
 | lam : ty -> tm -> tm
 | app : tm -> tm -> tm
 | unit : tm
@@ -13,9 +13,10 @@ inductive tm where
 instance : Ids tm where
   ids := tm.var
 
-@[simp] theorem ids_var x : tm.var x = ids x := rfl
+@[asimp]theorem ids_var x : tm.var x = ids x := rfl
 
-def tm.rename (ξ : Nat -> Nat) (m : tm) : tm :=
+@[asimp]
+def tm.rename (ξ : Var -> Var) (m : tm) : tm :=
   match m with
   | var x => var (ξ x)
   | lam a m => lam a (rename (upren ξ) m)
@@ -25,12 +26,12 @@ def tm.rename (ξ : Nat -> Nat) (m : tm) : tm :=
 instance : Rename tm where
   rename := tm.rename
 
-@[simp] theorem rename_ids ξ x : rename ξ (ids x) = @ids tm _ (ξ x) := rfl
-@[simp] theorem rename_lam ξ a m : rename ξ (tm.lam a m) = tm.lam a (rename (upren ξ) m) := rfl
-@[simp] theorem rename_app ξ m n : rename ξ (tm.app m n) = tm.app (rename ξ m) (rename ξ n) := rfl
-@[simp] theorem rename_unit ξ : rename ξ (tm.unit) = tm.unit := rfl
+@[asimp]theorem rename_ids ξ x : rename ξ (ids x) = @ids tm _ (ξ x) := rfl
+@[asimp]theorem rename_lam ξ a m : rename ξ (tm.lam a m) = tm.lam a (rename (upren ξ) m) := rfl
+@[asimp]theorem rename_app ξ m n : rename ξ (tm.app m n) = tm.app (rename ξ m) (rename ξ n) := rfl
+@[asimp]theorem rename_unit ξ : rename ξ (tm.unit) = tm.unit := rfl
 
-def tm.subst (σ : Nat -> tm) (m : tm) : tm :=
+def tm.subst (σ : Var -> tm) (m : tm) : tm :=
   match m with
   | var x => σ x
   | lam a m => lam a (subst (up σ) m)
@@ -40,185 +41,129 @@ def tm.subst (σ : Nat -> tm) (m : tm) : tm :=
 instance : Subst tm where
   subst := tm.subst
 
-@[simp] theorem subst_ids (σ : Nat -> tm) x : subst σ (ids x) = σ x := by rfl
-@[simp] theorem subst_lam σ a m : subst σ (tm.lam a m) = tm.lam a (subst (up σ) m) := by rfl
-@[simp] theorem subst_app σ m n : subst σ (tm.app m n) = tm.app (subst σ m) (subst σ n) := by rfl
-@[simp] theorem subst_unit σ : subst σ tm.unit = tm.unit := rfl
+@[asimp]theorem subst_ids (σ : Var -> tm) x : subst σ (ids x) = σ x := by rfl
+@[asimp]theorem subst_lam σ a m : subst σ (tm.lam a m) = tm.lam a (subst (up σ) m) := by rfl
+@[asimp]theorem subst_app σ m n : subst σ (tm.app m n) = tm.app (subst σ m) (subst σ n) := by rfl
+@[asimp]theorem subst_unit σ : subst σ tm.unit = tm.unit := rfl
 
-theorem up_upren (ξ : Nat -> Nat) :
+theorem up_upren (ξ : Var -> Var) :
   @up tm _ _ (ren ξ) = ren (upren ξ) := by
-  apply funext
-  intro x
-  cases x with
-  | zero => simp [upren, up, ren, scons, funcomp]
-  | succ => simp [upren, up, ren, scons, funcomp]
+  funext x; cases x <;> asimp
 
-theorem up_upren_n (ξ : Nat -> Nat) (n : Nat) :
+theorem up_upren_n (ξ : Var -> Var) (n : Var) :
   @upn tm _ _ n (ren ξ ) = ren (n.repeat upren ξ) := by
   induction n generalizing ξ with
-  | zero => simp [upn, Nat.repeat]
+  | zero =>
+    asimp[Nat.repeat]
   | succ n ih =>
-    simp[upn, Nat.repeat];
+    asimp[Nat.repeat]
     rw [<-up_upren]
-    rw [<-ih, <-upn]
+    rw [<-ih]
 
-@[simp] theorem rename_subst ξ (m : tm) : rename ξ m = m.[ren ξ] := by
+theorem tm.rename_subst ξ (m : tm) : rename ξ m = m.[ren ξ] := by
   induction m generalizing ξ with
-  | var x => simp [ren, funcomp]
+  | var x => simp[asimp]
   | lam a m ih =>
-    simp[up_upren]; rw[ih]
+    asimp[up_upren]; rw[ih]
   | app m n ihm ihn =>
-    simp
+    asimp
     constructor
     . apply ihm
     . apply ihn
-  | _ => simp
+  | _ => asimp
 
-@[simp] theorem up_shift (σ : Nat -> tm) :
-  up σ = ids 0 .: (σ @@ shift) := by
-  simp [up, scomp]
-  apply funext
-  intro x
+theorem up_ids : up ids = @ids tm _ := by
+  funext x
   cases x with
-  | zero => simp[scons]
-  | succ x =>
-    simp [scons, funcomp]
-    simp [rename_subst, shift]
+  | zero => asimp
+  | succ => asimp
 
-open Lean Elab Macro
-syntax "asimp" : tactic
-syntax "asimp" "at" ident : tactic
-macro_rules
-| `(tactic| asimp) =>
-  `(tactic| simp; repeat rw [<-up_shift])
-| `(tactic| asimp at $x:ident) =>
-  `(tactic| simp at $x:ident; repeat rw [<-up_shift] at $x:ident)
-
-@[simp] theorem ids_comp (σ : Nat -> tm) : ids @@ σ = σ := by rfl
-@[simp] theorem ids_shift : (@ids tm _ 0) .: shift = ids := by
-  apply funext
-  intro x
-  cases x with
-  | zero => simp[scons]
-  | succ x => simp[scons, shift, ren, funcomp]
-
-@[simp] theorem shift_scomp (m : tm) (σ : Nat -> tm) :
-  shift @@ (m .: σ) = σ := by
-  apply funext
-  intro x
-  simp[shift, ren]
-  simp[funcomp, scomp, scons]
-
-@[simp] theorem ids0_scons (σ : Nat -> tm) :
-  (ids 0).[σ] .: (shift @@ σ) = σ := by
-  apply funext
-  intro x
-  simp[scons]
-  cases x with
-  | zero => simp
-  | succ => simp[scomp, funcomp, shift, ren]
-
-@[simp] theorem subst_id (m : tm) :
+theorem tm.subst_id (m : tm) :
   m.[ids] = m := by
   induction m with
-  | var x => simp
+  | var x => asimp
   | lam a m ih =>
-    simp
+    asimp[up_ids]
     assumption
   | app m n ih1 ih2 =>
-    simp
+    asimp
     constructor <;> assumption
-  | unit => simp
+  | unit => asimp
 
-@[simp] theorem comp_ids (σ : Nat -> tm) : σ @@ ids = σ := by
-  apply funext
-  intro x
-  simp[scomp, funcomp]
-
-@[simp] theorem scons_scomp m (σ τ : Nat -> tm) :
-  (m .: σ) @@ τ = m.[τ] .: σ @@ τ := by
-  apply funext
-  intro x
-  cases x with
-  | zero => simp[scomp, funcomp, scons]
-  | succ => simp[scomp, funcomp, scons]
-
-theorem up_comp_ren_subst {T} [Ids T] [Rename T] (ξ : Nat -> Nat) (σ : Nat -> T) :
-  up (ξ @@@ σ) = upren ξ @@@ up σ := by
-  apply funext
-  intro x
+theorem up_comp_ren_subst {T} [Ids T] [Rename T] (ξ : Var -> Var) (σ : Var -> T) :
+  up (ξ >>> σ) = upren ξ >>> up σ := by
+  funext x
   cases x with
   | zero => rfl
-  | succ n => simp [up, scons, upren, funcomp]
+  | succ => asimp
 
-theorem ren_subst_comp ξ σ (m : tm) : m.[ren ξ].[σ] = m.[ξ @@@ σ] := by
+theorem ren_subst_comp ξ σ (m : tm) : m.[ren ξ].[σ] = m.[ξ >>> σ] := by
   induction m generalizing ξ σ with
   | var x => rfl
   | lam a m ih =>
-    simp [up_comp_ren_subst]
+    asimp[up_comp_ren_subst]
     rw [<- ih]
-    simp [<- up_upren]
+    simp [up_upren]
   | app m n ihm ihn =>
-    simp; constructor
+    asimp; constructor
     . rw [<- ihm]
     . rw [<- ihn]
-  | unit => simp
+  | unit => asimp
 
-theorem up_comp_subst_ren (σ : Nat -> tm) (ξ : Nat -> Nat) :
-  up (σ @@@ rename ξ) = up σ @@@ rename (upren ξ) := by
-  apply funext
-  intro x
+theorem up_comp_subst_ren (σ : Var -> tm) (ξ : Var -> Var) :
+  up (σ >>> rename ξ) = up σ >>> rename (upren ξ) := by
+  funext x
   cases x with
-  | zero => simp [ren, funcomp]
+  | zero => asimp
   | succ n =>
-    simp [up, scons, funcomp]
-    have h1 := ren_subst_comp Nat.succ (ren (upren ξ)) (σ n); simp at h1
-    have h2 := ren_subst_comp ξ (ren Nat.succ) (σ n); simp at h2
+    asimp[rename, tm.rename_subst]
+    have h1 := ren_subst_comp Nat.succ (ren (upren ξ)) (σ n); asimp at h1
+    have h2 := ren_subst_comp ξ (ren Nat.succ) (σ n); asimp at h2
     rw [h1, h2]; rfl
 
-theorem subst_ren_comp σ ξ (m : tm) : m.[σ].[ren ξ] = m.[σ @@@ rename ξ] := by
+theorem subst_ren_comp σ ξ (m : tm) : m.[σ].[ren ξ] = m.[σ >>> rename ξ] := by
   induction m generalizing σ ξ with
-  | var x => simp
+  | var x =>
+    asimp[rename, tm.rename_subst]
   | lam a m ih =>
     asimp;
     rw [up_upren]
     rw [ih]
     rw [<- up_comp_subst_ren]
   | app m n ihm ihn =>
-    simp; constructor
+    asimp; constructor
     . rw [<- ihm]
     . rw [<- ihn]
   | unit => rfl
 
-theorem up_comp (σ τ : Nat -> tm) : up (σ @@ τ) = up σ @@ up τ := by
+theorem up_comp (σ τ : Var -> tm) : up (σ >> τ) = up σ >> up τ := by
   apply funext
   intro x
   cases x with
   | zero =>
-    simp [up, scons, scomp, funcomp]
+    asimp
   | succ n =>
-    simp [up, scons, scomp, funcomp]
-    rw[<-up]
+    asimp[rename, tm.rename_subst]
     have h1 := subst_ren_comp τ Nat.succ (σ n)
     have h2 := ren_subst_comp Nat.succ (up τ) (σ n)
     rw [h1, h2]
     rfl
 
-@[simp] theorem subst_comp (σ τ : Nat -> tm) m : m.[σ].[τ] = m.[σ @@ τ] := by
+theorem tm.subst_comp (σ τ : Var -> tm) m : m.[σ].[τ] = m.[σ >> τ] := by
   induction m generalizing σ τ with
-  | var x => simp [scomp, funcomp]
+  | var x => asimp
   | lam a m ih =>
     asimp
     rw [ih]
-    rw [up_comp]
+    rw [<-up_comp]
   | app m n ihm ihn =>
-    simp; constructor
+    asimp; constructor
     . apply ihm
     . apply ihn
   | unit => rfl
 
-@[simp] theorem scomp_assoc (σ τ θ : Nat -> tm) :
-  (σ @@ τ) @@ θ = σ @@ (τ @@ θ) := by
-  apply funext
-  intro x
-  simp[scomp, funcomp]
+instance : SubstLemmas tm where
+  rename_subst := tm.rename_subst
+  subst_id := tm.subst_id
+  id_subst := by intros; asimp
+  subst_comp := tm.subst_comp
