Lamcalc.lean
@@ -1,5 +1,6 @@
 -- This module serves as the root of the `Lamcalc` library.
 -- Import modules here that should be built as part of the library.
+import Lamcalc.Attr
 import Lamcalc.ARS
 import Lamcalc.Basics
 import Lamcalc.Syntax
