Lamcalc/Attr.lean
@@ -1,0 +1,2 @@
+import Lean.Meta.Tactic.Simp
+register_simp_attr asimp
